Examples completely implemented.

src/QueryStructure/Automation/SearchTerms/RangeSearchTerms.v
@@ -1,75 +1,92 @@
 Require Import
+        Coq.FSets.FMapInterface
+        Coq.FSets.FMapFacts
+        Coq.FSets.FMapAVL
+        Coq.Structures.OrderedTypeEx
+        Fiat.Common.String_as_OT
+        Fiat.QueryStructure.Implementation.DataStructures.Bags.RangeTreeBags
         Fiat.QueryStructure.Specification.Representation.QueryStructureNotations
         Fiat.QueryStructure.Specification.SearchTerms.InRange
         Fiat.QueryStructure.Implementation.DataStructures.BagADT.IndexSearchTerms
         Fiat.QueryStructure.Automation.IndexSelection
-        Fiat.QueryStructure.Automation.Common.
+        Fiat.QueryStructure.Automation.Common
+        Fiat.QueryStructure.Implementation.DataStructures.Bags.CountingListBags
+        Fiat.QueryStructure.Implementation.DataStructures.Bags.BagsOfTuples
+.
 
 (* Instances for building indexes with make simple indexes. *)
 (* Every Kind of index is keyed on an inductive type with a single constructor*)
 Definition RangeIndex : string := "RangeIndex".
 
-(* This is our search term type. *)
-Record RangeSearchTerm
-       (heading : RawHeading)
-  :=
-    { RangeIndexSearchTerm : (option nat) * (option nat);
-      RangeItemSearchTerm : @RawTuple heading -> bool }.
+Ltac BuildLastRangeIndex
+     heading indices kind index k k_fail :=
+  let is_equality := eval compute in (string_dec kind RangeIndex) in
+      match is_equality with
+      | left _ => k
+                    (fun (search_term : prod (prod (option (Domain heading index)) (option (Domain heading index))) (@RawTuple heading -> bool))
+                         (tup : @RawTuple heading) =>
+                       match fst search_term with
+                       | (Some minRange, Some maxRange) =>
+                         if InRange_dec (GetAttributeRaw tup index) minRange maxRange then
+                           (snd search_term) tup
+                         else false
+                       | (None, Some maxRange) =>
+                         if le_dec (GetAttributeRaw tup index) maxRange then
+                           (snd search_term) tup
+                         else false
+                       | (Some minRange, None) =>
+                         if le_dec minRange (GetAttributeRaw tup index) then
+                           (snd search_term) tup
+                         else false
+                       | (None, None) => (snd search_term) tup
+                       end)
+      | right _ => k_fail heading indices kind index k
+      end.
 
-(* This builds the type of searchterms and the matching function on them *)
-Global Instance RangeIndexDenotation
-       (heading : RawHeading)
-       (index : @Attributes heading)
-       (projection : @RawTuple heading -> nat)
-: @IndexDenotation "RangeIndex" heading index :=
-  {| DenoteIndex := RangeSearchTerm heading; (* Pick search term type *)
-     MatchIndex search_term item := (* matching function : DenoteIndex -> RawTuple heading -> bool *)
-       match RangeIndexSearchTerm search_term with
-         | (Some minRange, Some maxRange) =>
-           if InRange_dec (projection item) minRange maxRange then
-             RangeItemSearchTerm search_term item
-           else false
-         | (None, Some maxRange) =>
-           if le_dec (projection item) maxRange then
-             RangeItemSearchTerm search_term item
-           else false
-         | (Some minRange, None) =>
-           if le_dec minRange (projection item) then
-             RangeItemSearchTerm search_term item
-           else false
-         | (_, _) => RangeItemSearchTerm search_term item
-       end |}.
-
-(* Extra type class magic for range indices. *)
-Hint Extern 10 (@IndexDenotation "RangeIndex" ?heading ?index) =>
-let index_domain := eval hnf in (@Domain heading index) in
-match index_domain with
-  | nat =>
-    apply (@RangeIndexDenotation
-             heading index
-             (fun tup => GetAttributeRaw tup index ))
-end
-: typeclass_instances.
+Ltac BuildEarlyRangeIndex
+     heading indices kind index matcher k k_fail :=
+  let is_equality := eval compute in (string_dec kind RangeIndex) in
+      match is_equality with
+      | left _ => k
+                    (fun (search_term : prod (prod (option (Domain heading index)) (option (Domain heading index))) (@RawTuple heading -> bool))
+                         (tup : @RawTuple heading) =>
+                       match fst search_term with
+                       | (Some minRange, Some maxRange) =>
+                         if InRange_dec (GetAttributeRaw tup index) minRange maxRange then
+                           matcher (snd search_term) tup
+                         else false
+                       | (None, Some maxRange) =>
+                         if le_dec (GetAttributeRaw tup index) maxRange then
+                           matcher (snd search_term)  tup
+                         else false
+                       | (Some minRange, None) =>
+                         if le_dec minRange (GetAttributeRaw tup index) then
+                           matcher (snd search_term) tup
+                         else false
+                       | (None, None) => matcher (snd search_term) tup
+                       end)
+      | right _ => k_fail heading indices kind index matcher k
+      end.
 
 Ltac matchRangeIndex qsSchema WhereClause k k_fail :=
   match WhereClause with
   | fun tups => (@?C2 tups) <= (@?C1 tups) <= _ =>
     TermAttributes C1 ltac:(fun Ridx1 attr1 =>
                               TermAttributes C2
-                              ltac:(fun Ridx2 attr2 =>
-                                      k (@InsertOccurence _ qsSchema Ridx1 (RangeIndex, attr1) (@InsertOccurence _ qsSchema Ridx2 (RangeIndex, attr2) (InitOccurence _)))))
+                                             ltac:(fun Ridx2 attr2 =>
+                                                     k (@InsertOccurence _ qsSchema Ridx1 (RangeIndex, attr1) (@InsertOccurence _ qsSchema Ridx2 (RangeIndex, attr2) (InitOccurence _)))))
 
   | fun tups => _ <= (@?C1 tups) <= (@?C2 tups) =>
     TermAttributes C1 ltac:(fun Ridx1 attr1 =>
                               TermAttributes C2
-                              ltac:(fun Ridx2 attr2 =>
-                                      k (@InsertOccurence _ qsSchema Ridx1 (RangeIndex, attr1) (@InsertOccurence _ qsSchema Ridx2 (RangeIndex, attr2) (InitOccurence _)))))
+                                             ltac:(fun Ridx2 attr2 =>
+                                                     k (@InsertOccurence _ qsSchema Ridx1 (RangeIndex, attr1) (@InsertOccurence _ qsSchema Ridx2 (RangeIndex, attr2) (InitOccurence _)))))
 
   | fun tups => (@?C1 tups) <= (@?C2 tups) =>
     TermAttributes C1 ltac:(fun Ridx1 attr1 =>
                               TermAttributes C2
                                              ltac:(fun Ridx2 attr2 =>
-                                      k (@InsertOccurence _ qsSchema Ridx1 (RangeIndex, attr1) (@InsertOccurence _ qsSchema Ridx2 (RangeIndex, attr2) (InitOccurence _)))))
+                                                     k (@InsertOccurence _ qsSchema Ridx1 (RangeIndex, attr1) (@InsertOccurence _ qsSchema Ridx2 (RangeIndex, attr2) (InitOccurence _)))))
 
   | fun tups => _ <= (@?C1 tups) =>
     TermAttributes C1 ltac:(fun Ridx attr =>
@@ -81,8 +98,8 @@ Ltac matchRangeIndex qsSchema WhereClause k k_fail :=
   end.
 
 Ltac RangeIndexUse SC F indexed_attrs f k k_fail :=
-match type of f with
-        (* Range Search Terms *)
+  match type of f with
+  (* Range Search Terms *)
   | forall a, {?X <= GetAttributeRaw _ ?fd <= ?Y} + {_} =>
     let H := fresh in
     assert (List.In (@Build_KindIndex SC "RangeIndex" fd) indexed_attrs) as H
@@ -101,95 +118,91 @@ match type of f with
     k ((@Build_KindIndex SC "RangeIndex" fd), (Some X, @None nat)) (fun _ : @RawTuple SC => true)
 
   | _ => k_fail SC F indexed_attrs f k
-end.
+  end.
 
 Ltac RangeIndexUse_dep SC F indexed_attrs visited_attrs f T k k_fail :=
-    match type of f with
-    (* Range Search Terms *)
-    | forall (a : ?Dom) b, { @?X a <= GetAttributeRaw _ ?fd <= @?Y a} + {_} =>
-      let H := fresh in
-          assert (List.In (@Build_KindIndex SC "RangeIndex" fd) indexed_attrs) as H
-          by (clear; simpl; intuition eauto); clear H;
-                              match eval simpl in
-                                    (in_dec fin_eq_dec fd visited_attrs) with
-                              | right _ => k (fd :: visited_attrs)
-                                             ((@Build_KindIndex SC "RangeIndex" fd), fun a : Dom => (Some (X a), Some (Y a)))
-                                             (fun (a : T) (_ : @RawTuple SC) => true)
-                              | left _ => k visited_attrs tt F
-                              end
+  match type of f with
+  (* Range Search Terms *)
+  | forall (a : ?Dom) b, { @?X a <= GetAttributeRaw _ ?fd <= @?Y a} + {_} =>
+    let H := fresh in
+    assert (List.In (@Build_KindIndex SC "RangeIndex" fd) indexed_attrs) as H
+        by (clear; simpl; intuition eauto); clear H;
+    match eval simpl in
+          (in_dec fin_eq_dec fd visited_attrs) with
+    | right _ => k (fd :: visited_attrs)
+                   ((@Build_KindIndex SC "RangeIndex" fd), fun a : Dom => (Some (X a), Some (Y a)))
+                   (fun (a : T) (_ : @RawTuple SC) => true)
+    | left _ => k visited_attrs tt F
+    end
 
-    | forall (a : ?Dom) b, { @?X a <= GetAttributeRaw _ ?fd} + {_} =>
-        let H := fresh in
-        assert (List.In (@Build_KindIndex SC "RangeIndex" fd) indexed_attrs) as H
-            by (clear; simpl; intuition eauto); clear H;
-        match eval simpl in
-              (in_dec fin_eq_dec fd visited_attrs) with
-          | right _ => k (fd :: visited_attrs)
-                         ((@Build_KindIndex SC "RangeIndex" fd), fun a : Dom => (Some (X a), @None nat))
-                         (fun (a : T) (_ : @RawTuple SC) => true)
-          | left _ => k visited_attrs tt F
-        end
+  | forall (a : ?Dom) b, { @?X a <= GetAttributeRaw _ ?fd} + {_} =>
+    let H := fresh in
+    assert (List.In (@Build_KindIndex SC "RangeIndex" fd) indexed_attrs) as H
+        by (clear; simpl; intuition eauto); clear H;
+    match eval simpl in
+          (in_dec fin_eq_dec fd visited_attrs) with
+    | right _ => k (fd :: visited_attrs)
+                   ((@Build_KindIndex SC "RangeIndex" fd), fun a : Dom => (Some (X a), @None nat))
+                   (fun (a : T) (_ : @RawTuple SC) => true)
+    | left _ => k visited_attrs tt F
+    end
 
-      | forall (a : ?Dom) b, {GetAttributeRaw _ ?fd <= (@?X a)} + {_} =>
-        let H := fresh in
-        assert (List.In (@Build_KindIndex SC "RangeIndex" fd) indexed_attrs) as H
-            by (clear; simpl; intuition eauto); clear H;
-        match eval simpl in
-              (in_dec fin_eq_dec fd visited_attrs) with
-          | right _ => k (fd :: visited_attrs)
-                         ((@Build_KindIndex SC "RangeIndex" fd), fun a : Dom => (@None nat, Some (X a)))
-                         (fun (a : T) (_ : @RawTuple SC) => true)
-          | left _ => k visited_attrs tt F
-        end
-      | _ => k_fail SC F indexed_attrs visited_attrs f T k
-    end.
+  | forall (a : ?Dom) b, {GetAttributeRaw _ ?fd <= (@?X a)} + {_} =>
+    let H := fresh in
+    assert (List.In (@Build_KindIndex SC "RangeIndex" fd) indexed_attrs) as H
+        by (clear; simpl; intuition eauto); clear H;
+    match eval simpl in
+          (in_dec fin_eq_dec fd visited_attrs) with
+    | right _ => k (fd :: visited_attrs)
+                   ((@Build_KindIndex SC "RangeIndex" fd), fun a : Dom => (@None nat, Some (X a)))
+                   (fun (a : T) (_ : @RawTuple SC) => true)
+    | left _ => k visited_attrs tt F
+    end
+  | _ => k_fail SC F indexed_attrs visited_attrs f T k
+  end.
 
 Ltac createLastRangeTerm f fds tail fs kind s k k_fail :=
   let is_equality := eval compute in (string_dec kind "RangeIndex") in
       match is_equality with
-        | left _ =>
-          (findMatchingTerm
-             fds kind s
-             ltac:(fun X => k {| RangeIndexSearchTerm := X;
-                                 RangeItemSearchTerm := tail |}))
-            || k {| RangeIndexSearchTerm := (@None nat, @None nat);
-                    RangeItemSearchTerm := tail |}
-        | _ => k_fail f fds tail fs kind s k
+      | left _ =>
+        (findMatchingTerm
+           fds kind s
+           ltac:(fun X => k (X, tail)))
+          || k ((@None nat, @None nat), tail)
+      | _ => k_fail f fds tail fs kind s k
       end.
 
 Ltac createLastRangeTerm_dep dom f fds tail fs kind s k k_fail :=
   let is_equality := eval compute in (string_dec kind "RangeIndex") in
       match is_equality with
-        | left _ =>
-          (findMatchingTerm
-             fds kind s
-             ltac:(fun X => k (fun x : dom => {| RangeIndexSearchTerm := X x;
-                                                 RangeItemSearchTerm := tail x |}))
-                    || k (fun x : dom => {| RangeIndexSearchTerm := (@None nat, @None nat);
-                                            RangeItemSearchTerm := tail x |}))
-        | _ => k_fail dom f fds tail fs kind s k
+      | left _ =>
+        (findMatchingTerm
+           fds kind s
+           ltac:(fun X => k (fun x : dom => (X x, tail x)))
+                  || k (fun x : dom => ((@None nat, @None nat), tail x )))
+      | _ => k_fail dom f fds tail fs kind s k
       end.
 
 Ltac createEarlyRangeTerm f fds tail fs kind EarlyIndex LastIndex rest s k k_fail :=
   let is_equality := eval compute in (string_dec kind "RangeIndex") in
       match is_equality with
-        | left _ =>
-          (findMatchingTerm
-             fds kind s
-             ltac:(fun X => k (X, rest)))
-            || k ((@None nat, @None nat), rest)
-        | _ => k_fail f fds tail fs kind EarlyIndex LastIndex rest s k
+      | left _ =>
+        (findMatchingTerm
+           fds kind s
+           ltac:(fun X => k (X, rest)))
+          || k ((@None nat, @None nat), rest)
+      | _ => k_fail f fds tail fs kind EarlyIndex LastIndex rest s k
       end.
 
 Ltac createEarlyRangeTerm_dep dom f fds tail fs kind EarlyIndex LastIndex rest s k k_fail :=
   let is_equality := eval compute in (string_dec kind "RangeIndex") in
       match is_equality with
-        | left _ =>
-          (findMatchingTerm
-             fds kind s
-             ltac:(fun X => k (fun x : dom => (X x, rest x))))
-            || k (fun x : dom => ((@None nat, @None nat), rest x))
-        | _ => k_fail dom f fds tail fs kind EarlyIndex LastIndex rest s k
+      | left _ =>
+        (findMatchingTerm
+           fds kind s
+           ltac:(fun X => k (fun x : dom => (X x, rest x))))
+          || k (fun x : dom => ((@None nat, @None nat), rest x))
+      | _ => k_fail dom f fds tail fs kind EarlyIndex LastIndex rest s k
       end.
 
 Ltac RangeIndexTactics f :=
@@ -197,3 +210,136 @@ Ltac RangeIndexTactics f :=
     matchRangeIndex
     RangeIndexUse createEarlyRangeTerm createLastRangeTerm
     RangeIndexUse_dep createEarlyRangeTerm_dep createLastRangeTerm_dep f.
+
+Module StringRangeTreeBag := RangeTreeBag String_as_OT.
+Module NatRangeTreeBag := RangeTreeBag Nat_as_OT.
+Module NRangeTreeBag := RangeTreeBag N_as_OT.
+Module ZRangeTreeBag := RangeTreeBag Z_as_OT.
+
+Definition NatRangeTreeBag'
+           (heading : RawHeading)
+           {BagType SearchTermType UpdateTermType : Type}
+           (TBag : Bag BagType (@RawTuple heading) SearchTermType UpdateTermType)
+           (projection : RawTuple -> NatRangeTreeBag.MoreXMapFacts.TKey)
+           (bupdate_transform : UpdateTermType -> RawTuple -> RawTuple)
+  : Bag (NatRangeTreeBag.RangeTreeBag (BagType := BagType)) (@RawTuple heading)
+        (option NatRangeTreeBag.MoreXMapFacts.TKey *
+         option NatRangeTreeBag.MoreXMapFacts.TKey * SearchTermType)
+        UpdateTermType :=
+  {| bempty            := NatRangeTreeBag.RangeTreeBag_bempty;
+     bfind_matcher    :=
+       fun (search_term : prod _ SearchTermType)
+           (tup : @RawTuple heading) =>
+         match fst search_term with
+         | (Some minRange, Some maxRange) =>
+           if InRange_dec (projection tup) minRange maxRange then
+             (bfind_matcher (snd search_term)) tup
+           else false
+         | (None, Some maxRange) =>
+           if le_dec (projection tup) maxRange then
+             (bfind_matcher (snd search_term)) tup
+           else false
+         | (Some minRange, None) =>
+           if le_dec minRange (projection tup) then
+             (bfind_matcher (snd search_term)) tup
+           else false
+         | (None, None) => (bfind_matcher (snd search_term)) tup
+         end;
+     bupdate_transform := bupdate_transform;
+
+     benumerate := NatRangeTreeBag.RangeTreeBag_benumerate TBag;
+     bfind      := NatRangeTreeBag.RangeTreeBag_bfind TBag;
+     binsert    := NatRangeTreeBag.RangeTreeBag_binsert TBag projection;
+     bcount     := NatRangeTreeBag.RangeTreeBag_bcount TBag;
+     bdelete    := NatRangeTreeBag.RangeTreeBag_bdelete TBag;
+     bupdate    := NatRangeTreeBag.RangeTreeBag_bupdate TBag |}.
+
+Lemma bfind_matcher_eq          (heading : RawHeading)
+      {BagType SearchTermType UpdateTermType : Type}
+      (TBag : Bag BagType (@RawTuple heading) SearchTermType UpdateTermType)
+      projection
+  : NatRangeTreeBag.RangeTreeBag_bfind_matcher TBag projection
+    = @bfind_matcher _ _ _ _ (NatRangeTreeBag' _ _ projection bupdate_transform).
+Proof.
+  repeat (apply functional_extensionality; intros).
+  destruct x as [[[st | ] [st' | ]] st''];
+    unfold NatRangeTreeBag.RangeTreeBag_bfind_matcher,
+    NatRangeTreeBag.Range_InRange; simpl;
+    unfold NatRangeTreeBag.X_le_dec; simpl;
+    unfold InRange_dec;
+    repeat first [
+             solve [ eauto ]
+           | match goal with
+             | |- appcontext[Nat_as_OT.compare ?st ?st'] =>
+               destruct (Nat_as_OT.compare st st'); simpl
+             | |- appcontext[le_dec ?st ?st'] =>
+               destruct (le_dec st st'); simpl
+             end
+           | progress (unfold Nat_as_OT.lt, Nat_as_OT.eq in *; omega)
+           ].
+Qed.
+
+Instance NatRangeTreeBagCorrect
+         (heading : RawHeading)
+         {BagType SearchTermType UpdateTermType : Type}
+         (TBag : Bag BagType (@RawTuple heading) SearchTermType UpdateTermType)
+         (RepInv : BagType -> Prop)
+         (ValidUpdate : UpdateTermType -> Prop)
+         (CorrectTBag : CorrectBag RepInv ValidUpdate TBag)
+         (projection : RawTuple -> NatRangeTreeBag.MoreXMapFacts.TKey)
+  : @CorrectBag _ _ _
+                UpdateTermType
+                (NatRangeTreeBag.RangeTreeBag_RepInv _ RepInv projection)
+                (NatRangeTreeBag.RangeTreeBag_ValidUpdate _ ValidUpdate projection)
+                (@NatRangeTreeBag' heading BagType  SearchTermType UpdateTermType TBag projection bupdate_transform) :=
+  { bempty_RepInv     := @NatRangeTreeBag.RangeTreeBag_Empty_RepInv BagType RawTuple SearchTermType UpdateTermType TBag RepInv projection;
+    binsert_RepInv    := NatRangeTreeBag.RangeTreeBag_binsert_Preserves_RepInv CorrectTBag (projection := projection);
+    bdelete_RepInv    := NatRangeTreeBag.RangeTreeBag_bdelete_Preserves_RepInv CorrectTBag (projection := projection);
+    bupdate_RepInv    := NatRangeTreeBag.RangeTreeBag_bupdate_Preserves_RepInv CorrectTBag (projection := projection);
+
+    binsert_enumerate := NatRangeTreeBag.RangeTreeBag_BagInsertEnumerate CorrectTBag (projection := projection);
+    benumerate_empty  := NatRangeTreeBag.RangeTreeBag_BagEnumerateEmpty (TBag := TBag)
+  }.
+destruct (bfind_matcher_eq heading TBag projection);
+  apply (NatRangeTreeBag.RangeTreeBag_BagFindCorrect CorrectTBag (projection := projection)).
+destruct (bfind_matcher_eq heading TBag projection);
+  apply (NatRangeTreeBag.RangeTreeBag_BagCountCorrect CorrectTBag (projection := projection)).
+destruct (bfind_matcher_eq heading TBag projection);
+  apply (NatRangeTreeBag.RangeTreeBag_BagDeleteCorrect CorrectTBag (projection := projection)).
+destruct (bfind_matcher_eq heading TBag projection);
+  apply (NatRangeTreeBag.RangeTreeBag_BagUpdateCorrect CorrectTBag (projection := projection)).
+Qed.
+
+
+Ltac BuildLastRangeTreeBag heading AttrList AttrKind AttrIndex k k_fail :=
+  let is_equality := eval compute in (string_dec AttrKind "RangeIndex") in
+      match is_equality with
+      | left _ =>
+        let AttrType := eval compute in (Domain heading AttrIndex) in
+            match AttrType with
+            | nat =>
+              k (@NatRangeTreeBagCorrect _ _ _ _ _ _ _
+                                         (@CountingListAsCorrectBag
+                                            (@RawTuple heading)
+                                            (IndexedTreeUpdateTermType heading)
+                                            (IndexedTreebupdate_transform heading))
+                                         (fun x => GetAttributeRaw (heading := heading) x AttrIndex))
+
+            end
+      | right _ => k_fail heading AttrList AttrKind AttrIndex k
+      end.
+
+Ltac BuildEarlyRangeTreeBag heading AttrList AttrKind AttrIndex subtree k k_fail :=
+  let is_equality := eval compute in (string_dec AttrKind "RangeIndex") in
+      match is_equality with
+      | left _ =>
+        let AttrType := eval compute in (Domain heading AttrIndex) in
+            match AttrType with
+            | nat =>
+              k (@NatRangeTreeBagCorrect _ _ _ _ _ _ _
+                                         subtree
+                                         (fun x => GetAttributeRaw (heading := heading) x AttrIndex))
+
+            end
+      | right _ => k_fail heading AttrList AttrKind AttrIndex subtree k
+      end.
