src/QueryStructure/Automation/QSImplementation.v
@@ -9,11 +9,11 @@ Require Export Fiat.Common.ilist3_pair
 
 Ltac list_of_evar B As k :=
   match As with
-    | nil => k (@nil B)
-    | cons ?a ?As' =>
-      makeEvar B ltac:(fun b =>
-                         list_of_evar
-                           B As' ltac:(fun Bs => k (cons b Bs)))
+  | nil => k (@nil B)
+  | cons ?a ?As' =>
+    makeEvar B ltac:(fun b =>
+                       list_of_evar
+                         B As' ltac:(fun Bs => k (cons b Bs)))
   end.
 
 Lemma ValidUpdateCorrect
@@ -96,81 +96,81 @@ Definition LookupQSDelegateImpls' {n}
                                (BagApplyUpdateTerm SearchTerm)))
                 SearchTerms)
   : forall (idx : Fin.t n),
-      refineADT
-        (Build_IndexedQueryStructure_Impl_Specs SearchTerms idx)
-        (ComputationalADT.LiftcADT (projT1 (i3th2 DelegateImpls idx))).
-  Proof.
-    intro.
-    unfold Build_IndexedQueryStructure_Impl_Specs.
-    revert schemas SearchTerms DelegateImpls.
-    induction idx.
-    - intro; pattern n, schemas; eapply Vector.caseS; simpl.
-      intros; eapply (projT2 (prim_fst DelegateImpls)).
-    - intro schemas; revert idx IHidx;
-      pattern n, schemas; eapply Vector.caseS.
-      intros; eapply IHidx.
-  Defined.
+    refineADT
+      (Build_IndexedQueryStructure_Impl_Specs SearchTerms idx)
+      (ComputationalADT.LiftcADT (projT1 (i3th2 DelegateImpls idx))).
+Proof.
+  intro.
+  unfold Build_IndexedQueryStructure_Impl_Specs.
+  revert schemas SearchTerms DelegateImpls.
+  induction idx.
+  - intro; pattern n, schemas; eapply Vector.caseS; simpl.
+    intros; eapply (projT2 (prim_fst DelegateImpls)).
+  - intro schemas; revert idx IHidx;
+    pattern n, schemas; eapply Vector.caseS.
+    intros; eapply IHidx.
+Defined.
 
-  Ltac BuildQSDelegateSigs QSImpl :=
-    let p := eval unfold QSImpl in QSImpl in
-        let p := eval simpl in (Sharpened_DelegateSigs p) in
-            match p with
-              Build_IndexedQueryStructure_Impl_Sigs ?SearchTerms =>
-              pose SearchTerms
-            end;
-          repeat match goal with
-                 | H : ilist _ (?sch :: ?schemas')
-                   |- ilist _ (?sch :: ?schemas') =>
-                   let SearchTerm := fresh "SearchTerm" in
-                   econstructor 1;
-                     [let SearchTerm := eval simpl in (ilist_hd H) in
-                          exact SearchTerm |
-                      let SearchTerm := eval simpl in (ilist_tl H) in
-                          pose SearchTerm; clear H ]
-                 | |- _ => econstructor 2
-                 end.
+Ltac BuildQSDelegateSigs QSImpl :=
+  let p := eval unfold QSImpl in QSImpl in
+      let p := eval simpl in (Sharpened_DelegateSigs p) in
+          match p with
+            Build_IndexedQueryStructure_Impl_Sigs ?SearchTerms =>
+            pose SearchTerms
+          end;
+        repeat match goal with
+               | H : ilist _ (?sch :: ?schemas')
+                 |- ilist _ (?sch :: ?schemas') =>
+                 let SearchTerm := fresh "SearchTerm" in
+                 econstructor 1;
+                   [let SearchTerm := eval simpl in (ilist_hd H) in
+                        exact SearchTerm |
+                    let SearchTerm := eval simpl in (ilist_tl H) in
+                        pose SearchTerm; clear H ]
+               | |- _ => econstructor 2
+               end.
 
 
 Ltac BuildQSDelegateReps QSImpl :=
   let p := eval unfold QSImpl in QSImpl in
       let p := eval simpl in (Sharpened_DelegateSigs p) in
           match p with
-              Build_IndexedQueryStructure_Impl_Sigs ?SearchTerms =>
-              pose SearchTerms
+            Build_IndexedQueryStructure_Impl_Sigs ?SearchTerms =>
+            pose SearchTerms
           end;
-          repeat match goal with
-                   | H : ilist _ (?sch :: ?schemas')
-                     |- ilist _ (?sch :: ?schemas') =>
-               let SearchTerm := fresh "SearchTerm" in
-               econstructor 1;
-                 [let SearchTerm := eval simpl in (BagSearchTermType (ilist_hd H)) in
-                      match SearchTerm
-                      with
+        repeat match goal with
+               | H : ilist _ (?sch :: ?schemas')
+                 |- ilist _ (?sch :: ?schemas') =>
+                 let SearchTerm := fresh "SearchTerm" in
+                 econstructor 1;
+                   [let SearchTerm := eval simpl in (BagSearchTermType (ilist_hd H)) in
+                        match SearchTerm
+                        with
                         | BuildIndexSearchTerm ?AttrList =>
-                           pose AttrList;
-                             clear H;
-                             list_of_evar (@ProperAttribute (schemaHeading (relSchema sch))) AttrList
-                             ltac:(fun PAttrList =>
-                                     assert (map BagsOfTuples.Attribute PAttrList = AttrList)
-                                     by (simpl; repeat f_equal;
-                                         match goal with
-                                             |- @BagsOfTuples.Attribute ?heading ?h = ?g =>
-                                             instantiate (1 := @Build_ProperAttribute heading g _);
-                                             first [instantiate (1 := inright (eq_refl _))
-                                                   | instantiate (1 := inleft (inright (eq_refl _)))
-                                                   | instantiate (1 := inleft (inleft (right (eq_refl _))))
-                                                   | instantiate (1 := inleft (inleft (left (eq_refl _))))
-                                                   ]; reflexivity
-                                         end);
-                                   let p := eval simpl in (@NestedTreeFromAttributes _ PAttrList)
-                               in exact p)
+                          pose AttrList;
+                            clear H;
+                            list_of_evar (@ProperAttribute (schemaHeading (relSchema sch))) AttrList
+                                         ltac:(fun PAttrList =>
+                                                 assert (map BagsOfTuples.Attribute PAttrList = AttrList)
+                                                 by (simpl; repeat f_equal;
+                                                     match goal with
+                                                       |- @BagsOfTuples.Attribute ?heading ?h = ?g =>
+                                                       instantiate (1 := @Build_ProperAttribute heading g _);
+                                                       first [instantiate (1 := inright (eq_refl _))
+                                                             | instantiate (1 := inleft (inright (eq_refl _)))
+                                                             | instantiate (1 := inleft (inleft (right (eq_refl _))))
+                                                             | instantiate (1 := inleft (inleft (left (eq_refl _))))
+                                                             ]; reflexivity
+                                                     end);
+                                               let p := eval simpl in (@NestedTreeFromAttributes _ PAttrList)
+                                                 in exact p)
 
-                                    (* Other SearchTerm types go here. *)
-                      end
-                 | let SearchTerm := eval simpl in (ilist_tl H) in
-                       pose SearchTerm; clear H ]
-             | |- _ => econstructor 2
-           end.
+                                                (* Other SearchTerm types go here. *)
+                        end
+                   | let SearchTerm := eval simpl in (ilist_tl H) in
+                         pose SearchTerm; clear H ]
+               | |- _ => econstructor 2
+               end.
 
 (*Ltac BuildQSDelegateImpls QSImpl :=
       repeat match goal with
@@ -204,149 +204,162 @@ Ltac BuildQSDelegateReps QSImpl :=
                                                                      (@NestedTreeFromAttributesAsBag' _ PAttrList))) in clear H; exact p )
       end. *)
 
-  Ltac BuildQSIndexedBag heading AttrList k :=
-    match AttrList with
-      | ?Attr :: [ ] =>
-        let AttrKind := eval simpl in (KindIndexKind Attr) in
-            let AttrIndex := eval simpl in (KindIndexIndex Attr) in
-                let is_equality := eval compute in (string_dec AttrKind "EqualityIndex") in
+Ltac BuildQSIndexedBag heading AttrList BuildEarlyBag BuildLastBag k :=
+  match AttrList with
+  | ?Attr :: [ ] =>
+    let AttrKind := eval simpl in (KindIndexKind Attr) in
+        let AttrIndex := eval simpl in (KindIndexIndex Attr) in
+            let is_equality := eval compute in (string_dec AttrKind "EqualityIndex") in
 
-                    match is_equality with
-                  | left _ =>
-                    let AttrType := eval compute in (Domain heading AttrIndex) in
-                        match AttrType with
-                          | BinNums.N =>
-                            k (@NTreeBag.IndexedBagAsCorrectBag
-                                 _ _ _ _ _ _ _
-                                 (@CountingListAsCorrectBag
-                                    (@RawTuple heading)
-                                    (IndexedTreeUpdateTermType heading)
-                                    (IndexedTreebupdate_transform heading))
-                                 (fun x => GetAttributeRaw (heading := heading) x AttrIndex)
-                                 )
-                          | BinNums.Z =>
-                            k (@ZTreeBag.IndexedBagAsCorrectBag
-                                 _ _ _ _ _ _ _
-                                 (@CountingListAsCorrectBag
-                                    (@RawTuple heading)
-                                    (IndexedTreeUpdateTermType heading)
-                                    (IndexedTreebupdate_transform heading))
-                                 (fun x => GetAttributeRaw (heading := heading) x AttrIndex)
-                              )
-                          | nat =>
-                            k (@NatTreeBag.IndexedBagAsCorrectBag
-                                 _ _ _ _ _ _ _
-                                 (@CountingListAsCorrectBag
-                                    (@RawTuple heading)
-                                    (IndexedTreeUpdateTermType heading)
-                                    (IndexedTreebupdate_transform heading))
-                                 (fun x => GetAttributeRaw (heading := heading) x AttrIndex)
-                              )
-                          | string =>
-                            k (@StringTreeBag.IndexedBagAsCorrectBag
-                                 _ _ _ _ _ _ _
-                                 (@CountingListAsCorrectBag
-                                    (@RawTuple heading)
-                                    (IndexedTreeUpdateTermType heading)
-                                    (IndexedTreebupdate_transform heading))
-                                 (fun x => GetAttributeRaw (heading := heading) x AttrIndex)
-                              )
-                        end
-                    end
-      | ?Attr :: ?AttrList' =>
-        let AttrKind := eval simpl in (KindIndexKind Attr) in
-            let AttrIndex := eval simpl in (KindIndexIndex Attr) in
-                let is_equality := eval compute in (string_dec AttrKind "EqualityIndex") in
                 match is_equality with
-                  | left _ =>
-                    let AttrType := eval compute in (Domain heading AttrIndex) in
-                        match AttrType with
-                          | BinNums.N =>
-                            BuildQSIndexedBag
-                              heading
-                              AttrList'
-                              ltac:(fun subtree =>
-                                      k (@NTreeBag.IndexedBagAsCorrectBag
-                                           _ _ _ _ _ _ _ subtree
-                                           (fun x => GetAttributeRaw (heading := heading) x AttrIndex)))
-                          | BinNums.Z =>
-                            BuildQSIndexedBag
-                              heading
-                              AttrList'
-                              (fun x => GetAttributeRaw x AttrIndex)
-                              ltac:(fun subtree =>
-                                      k (@ZTreeBag.IndexedBagAsCorrectBag
-                                           _ _ _ _ _ _ _ subtree
-                                           (fun x => GetAttributeRaw (heading := heading) x AttrIndex)))
-                          | nat =>
-                            BuildQSIndexedBag
-                              heading
-                              AttrList'
-                              ltac:(fun subtree =>
-                                      k (@NatTreeBag.IndexedBagAsCorrectBag
-                                           _ _ _ _ _ _ _ subtree
-                                           (fun x => GetAttributeRaw (heading := heading) x AttrIndex)))
-                          | string =>
-                            BuildQSIndexedBag
-                              heading
-                              AttrList'
-                              ltac:(fun subtree =>
-                                      k (@StringTreeBag.IndexedBagAsCorrectBag
-                                           _ _ _ _ _ _ _ subtree
-                                           (fun x => GetAttributeRaw (heading := heading) x AttrIndex)))
-                        end
+                | left _ =>
+                  let AttrType := eval compute in (Domain heading AttrIndex) in
+                      match AttrType with
+                      | BinNums.N =>
+                        k (@NTreeBag.IndexedBagAsCorrectBag
+                             _ _ _ _ _ _ _
+                             (@CountingListAsCorrectBag
+                                (@RawTuple heading)
+                                (IndexedTreeUpdateTermType heading)
+                                (IndexedTreebupdate_transform heading))
+                             (fun x => GetAttributeRaw (heading := heading) x AttrIndex)
+                          )
+                      | BinNums.Z =>
+                        k (@ZTreeBag.IndexedBagAsCorrectBag
+                             _ _ _ _ _ _ _
+                             (@CountingListAsCorrectBag
+                                (@RawTuple heading)
+                                (IndexedTreeUpdateTermType heading)
+                                (IndexedTreebupdate_transform heading))
+                             (fun x => GetAttributeRaw (heading := heading) x AttrIndex)
+                          )
+                      | nat =>
+                        k (@NatTreeBag.IndexedBagAsCorrectBag
+                             _ _ _ _ _ _ _
+                             (@CountingListAsCorrectBag
+                                (@RawTuple heading)
+                                (IndexedTreeUpdateTermType heading)
+                                (IndexedTreebupdate_transform heading))
+                             (fun x => GetAttributeRaw (heading := heading) x AttrIndex)
+                          )
+                      | string =>
+                        k (@StringTreeBag.IndexedBagAsCorrectBag
+                             _ _ _ _ _ _ _
+                             (@CountingListAsCorrectBag
+                                (@RawTuple heading)
+                                (IndexedTreeUpdateTermType heading)
+                                (IndexedTreebupdate_transform heading))
+                             (fun x => GetAttributeRaw (heading := heading) x AttrIndex)
+                          )
+                      end
+                | right _ =>
+                  BuildLastBag heading AttrList AttrKind AttrIndex k
                 end
-    end.
+  | ?Attr :: ?AttrList' =>
+    let AttrKind := eval simpl in (KindIndexKind Attr) in
+        let AttrIndex := eval simpl in (KindIndexIndex Attr) in
+            let is_equality := eval compute in (string_dec AttrKind "EqualityIndex") in
+                match is_equality with
+                | left _ =>
+                  let AttrType := eval compute in (Domain heading AttrIndex) in
+                      match AttrType with
+                      | BinNums.N =>
+                        BuildQSIndexedBag
+                          heading AttrList'
+                          BuildEarlyBag BuildLastBag
+                          ltac:(fun subtree =>
+                                  k (@NTreeBag.IndexedBagAsCorrectBag
+                                       _ _ _ _ _ _ _ subtree
+                                       (fun x => GetAttributeRaw (heading := heading) x AttrIndex)))
+                      | BinNums.Z =>
+                        BuildQSIndexedBag
+                          heading AttrList'
+                          BuildEarlyBag BuildLastBag
+                          (fun x => GetAttributeRaw x AttrIndex)
+                          ltac:(fun subtree =>
+                                  k (@ZTreeBag.IndexedBagAsCorrectBag
+                                       _ _ _ _ _ _ _ subtree
+                                       (fun x => GetAttributeRaw (heading := heading) x AttrIndex)))
+                      | nat =>
+                        BuildQSIndexedBag
+                          heading AttrList'
+                          BuildEarlyBag BuildLastBag
+                          ltac:(fun subtree =>
+                                  k (@NatTreeBag.IndexedBagAsCorrectBag
+                                       _ _ _ _ _ _ _ subtree
+                                       (fun x => GetAttributeRaw (heading := heading) x AttrIndex)))
+                      | string =>
+                        BuildQSIndexedBag
+                          heading AttrList'
+                          BuildEarlyBag BuildLastBag
+                          ltac:(fun subtree =>
+                                  k (@StringTreeBag.IndexedBagAsCorrectBag
+                                       _ _ _ _ _ _ _ subtree
+                                       (fun x => GetAttributeRaw (heading := heading) x AttrIndex)))
+                      end
+                | right _ =>
+                  BuildQSIndexedBag
+                    heading AttrList'
+                    BuildEarlyBag BuildLastBag
+                    ltac:(fun subtree =>
+                            k (BuildEarlyBag
+                                 heading AttrList AttrKind AttrIndex subtree k))
+                end
+  end.
 
-
-  Ltac BuildQSIndexedBags SearchTerms k :=
-    match SearchTerms with
-      | @icons3 _ _ ?heading _ ?headings' ?SearchTerm
-                ?SeachTerms'
-        =>
-        let BagSearchTermType' := eval simpl in (BagSearchTermType SearchTerm) in
-            let AttrList' := match BagSearchTermType' with
-                             | BuildIndexSearchTerm ?AttrList => AttrList
-                             end in
-            BuildQSIndexedBags
-              SeachTerms'
-              ltac:(fun Bags =>
-                      BuildQSIndexedBag heading
-                                        AttrList'
-                                        ltac:(fun Bag => k (i3cons2
-                                                              (C := (fun sch (SearchTerm : SearchUpdateTerms sch) =>
-                   FullySharpened
-                     (@BagSpec (@RawTuple sch)
-                               (BagSearchTermType SearchTerm)
-                               (BagUpdateTermType SearchTerm)
-                               (BagMatchSearchTerm SearchTerm)
-                               (BagApplyUpdateTerm SearchTerm))))
-                                                              (b := SearchTerm)
-                                                              (@SharpenedBagImpl _ _ _ _ _ _ (fun _ => false) _ Bag (fun a b => ValidUpdateCorrect _ b)) Bags)))
-      | inil3 => k (i3nil2
-                      (C := fun heading (SearchTerm : SearchUpdateTerms heading) =>
-                         FullySharpened
-                           (@BagSpec (@RawTuple heading)
-                                     (BagSearchTermType SearchTerm)
-                                     (BagUpdateTermType SearchTerm)
-                                     (BagMatchSearchTerm SearchTerm)
-                                     (BagApplyUpdateTerm SearchTerm))))
-    end.
-
-    Ltac BuildQSIndexedBags' :=
-    repeat match goal with
-             H := BuildIndexSearchTerm _ |- _ => subst H
-           end;
-    match goal with
-        |- context [@Build_IndexedQueryStructure_Impl_Sigs _ ?indices ?SearchTerms _] =>
+Ltac BuildQSIndexedBags SearchTerms BuildEarlyBags BuildLastBags k :=
+  match SearchTerms with
+  | @icons3 _ _ ?heading _ ?headings' ?SearchTerm
+            ?SeachTerms'
+    =>
+    let BagSearchTermType' := eval simpl in (BagSearchTermType SearchTerm) in
+        let AttrList' := match BagSearchTermType' with
+                         | BuildIndexSearchTerm ?AttrList => AttrList
+                         end in
         BuildQSIndexedBags
-          SearchTerms
+          SeachTerms' BuildEarlyBags BuildLastBags
           ltac:(fun Bags =>
-                  let Impls := fresh in
-                  pose proof (@LookupQSDelegateImpls' _ indices SearchTerms Bags) as Impls; unfold  Update_Build_IndexedQueryStructure_Impl_cRep,
-                                                                                            Update_Iterate_Dep_Type in Impls; simpl in Impls;
-               apply Impls)
-    end.
+                  BuildQSIndexedBag
+                    heading AttrList'
+                    BuildEarlyBags BuildLastBags
+                    ltac:(fun Bag => k (i3cons2
+                                          (C := (fun sch (SearchTerm : SearchUpdateTerms sch) =>
+                                                   FullySharpened
+                                                     (@BagSpec (@RawTuple sch)
+                                                               (BagSearchTermType SearchTerm)
+                                                               (BagUpdateTermType SearchTerm)
+                                                               (BagMatchSearchTerm SearchTerm)
+                                                               (BagApplyUpdateTerm SearchTerm))))
+                                          (b := SearchTerm)
+                                          (@SharpenedBagImpl _ _ _ _ _ _ (fun _ => false) _ Bag (fun a b => ValidUpdateCorrect _ b)) Bags)))
+  | inil3 => k (i3nil2
+                  (C := fun heading (SearchTerm : SearchUpdateTerms heading) =>
+                          FullySharpened
+                            (@BagSpec (@RawTuple heading)
+                                      (BagSearchTermType SearchTerm)
+                                      (BagUpdateTermType SearchTerm)
+                                      (BagMatchSearchTerm SearchTerm)
+                                      (BagApplyUpdateTerm SearchTerm))))
+  end.
+
+Ltac BuildQSIndexedBags' BuildEarlyBags BuildLastBags :=
+  repeat match goal with
+           H := BuildIndexSearchTerm _ |- _ => subst H
+         end;
+  match goal with
+    |- context [@Build_IndexedQueryStructure_Impl_Sigs _ ?indices ?SearchTerms _] =>
+    BuildQSIndexedBags
+      SearchTerms BuildEarlyBags BuildLastBags
+      ltac:(fun Bags =>
+              let Impls := fresh in
+              pose proof (@LookupQSDelegateImpls' _ indices SearchTerms Bags) as Impls; unfold  Update_Build_IndexedQueryStructure_Impl_cRep,
+                                                                                        Update_Iterate_Dep_Type in Impls; simpl in Impls;
+            apply Impls
+           )
+  end.
+
+Ltac BuildLastEqualityBag heading AttrList AttrKind AttrIndex k := fail.
+Ltac BuildEarlyEqualityBag heading AttrList AttrKind AttrIndex subtree k := fail.
 
 Arguments LookupQSDelegateReps _ _ _ / .
 Arguments LookupQSDelegateImpls _ _ _ _ _ _ / .
