src/QueryStructure/Automation/SearchTerms/InclusionSearchTerms.v
@@ -4,42 +4,30 @@ Require Import
         Fiat.QueryStructure.Specification.SearchTerms.ListInclusion
         Fiat.QueryStructure.Implementation.DataStructures.BagADT.IndexSearchTerms
         Fiat.QueryStructure.Automation.IndexSelection
-        Fiat.QueryStructure.Automation.Common.
+        Fiat.QueryStructure.Automation.Common
+        Fiat.QueryStructure.Implementation.DataStructures.Bags.CountingListBags
+        Fiat.QueryStructure.Implementation.DataStructures.Bags.BagsOfTuples.
 
 (* Instances for building indexes with make simple indexes. *)
 (* Every Kind of index is keyed on an inductive type with a single constructor*)
 Local Open Scope string_scope.
 Definition InclusionIndex : string := "InclusionIndex".
 
-(* This is our search term type. *)
-Record InvertedSearchTerm
-       (heading : RawHeading)
-  :=
-    { IndexSearchTerm : list string;
-      ItemSearchTerm : @RawTuple heading -> bool }.
-
-(* This builds the type of searchterms and the matching function on them *)
-Global Instance InvertedIndexDenotation
-       (heading : RawHeading)
-       (index : @Attributes heading)
-       (projection : @RawTuple heading -> list string)
-: @IndexDenotation "InclusionIndex" heading index :=
-  {| DenoteIndex := InvertedSearchTerm heading; (* Pick search term type *)
-     MatchIndex search_term item := (* matching function : DenoteIndex -> Tuple heading -> bool *)
-       if IncludedIn_dec (IndexSearchTerm search_term) (projection item) then
-         ItemSearchTerm search_term item
-       else false |}.
-
-(* Extra type class magic for inverted indices. *)
-Hint Extern 10 (@IndexDenotation "InclusionIndex" ?heading ?index) =>
-let index_domain := eval hnf in (@Domain heading index) in
-match index_domain with
-  | list string =>
-    apply (@InvertedIndexDenotation
-             heading index
-             (fun tup => GetAttributeRaw tup index ))
-end
-: typeclass_instances.
+Ltac BuildLastInclusionIndex
+     heading indices kind index k k_fail :=
+  let is_equality := eval compute in (string_dec kind InclusionIndex) in
+      let A := eval compute in (Domain heading index) in
+          let A' := match A with | list ?A' => A' end in
+          match is_equality with
+          | left _ => k
+                        (fun (search_term : prod (Domain heading index) (@RawTuple heading -> bool)) (tup : @RawTuple heading) =>
+                           andb (if IncludedIn_dec (X := A')
+                                                   (fst search_term) (GetAttributeRaw tup index) then
+                                   true
+                                 else false)
+                                (snd search_term tup))
+          | right _ => k_fail heading indices kind index k
+          end.
 
 Ltac matchInclusionIndex qsSchema WhereClause k k_fail :=
   match WhereClause with
@@ -50,15 +38,15 @@ Ltac matchInclusionIndex qsSchema WhereClause k k_fail :=
   end.
 
 Ltac InclusionIndexUse SC F indexed_attrs f k k_fail :=
-     match type of f with
-       (* Inclusion Search Terms *)
-       | forall a, {IncludedIn ?X (GetAttributeRaw _ ?fd)} + {_} =>
-          let H := fresh in
-          assert (List.In (@Build_KindIndex SC "InclusionIndex" fd) indexed_attrs) as H
-              by (clear; subst_all; simpl; intuition eauto); clear H;
-            k (@Build_KindIndex SC "InclusionIndex" fd, X) (fun _ : @RawTuple SC => true)
-       | _ => k_fail SC F indexed_attrs f k
-     end.
+  match type of f with
+  (* Inclusion Search Terms *)
+  | forall a, {IncludedIn ?X (GetAttributeRaw _ ?fd)} + {_} =>
+    let H := fresh in
+    assert (List.In (@Build_KindIndex SC "InclusionIndex" fd) indexed_attrs) as H
+        by (clear; subst_all; simpl; intuition eauto); clear H;
+    k (@Build_KindIndex SC "InclusionIndex" fd, X) (fun _ : @RawTuple SC => true)
+  | _ => k_fail SC F indexed_attrs f k
+  end.
 
 Ltac InclusionIndexUse_dep SC F indexed_attrs visited_attrs f T k k_fail :=
   match type of f with
@@ -68,60 +56,56 @@ Ltac InclusionIndexUse_dep SC F indexed_attrs visited_attrs f T k k_fail :=
         by (clear; subst_all; simpl; intuition eauto); clear H;
     match eval simpl in
           (in_dec fin_eq_dec fd visited_attrs) with
-            | right _ => k (fd :: visited_attrs)
-                           (@Build_KindIndex SC "InclusionIndex" fd, X)
-                           (fun (a : T) (_ : @RawTuple SC) => true)
-            | left _ => k visited_attrs tt F
-          end
-    | _ => k_fail SC F indexed_attrs visited_attrs f T k
+    | right _ => k (fd :: visited_attrs)
+                   (@Build_KindIndex SC "InclusionIndex" fd, X)
+                   (fun (a : T) (_ : @RawTuple SC) => true)
+    | left _ => k visited_attrs tt F
+    end
+  | _ => k_fail SC F indexed_attrs visited_attrs f T k
   end.
 
 Ltac createLastInclusionTerm f fds tail fs kind s k k_fail :=
   let is_equality := eval compute in (string_dec kind "InclusionIndex") in
       match is_equality with
-        | left _ =>
-          (findMatchingTerm
-             fds kind s
-             ltac:(fun X => k {| IndexSearchTerm := X;
-                                 ItemSearchTerm := tail |}))
-            || k {| IndexSearchTerm := nil;
-                    ItemSearchTerm := tail |}
-        | _ => k_fail f fds tail fs kind s k
+      | left _ =>
+        (findMatchingTerm
+           fds kind s
+           ltac:(fun X => k (X : (Domain f s), tail)))
+          || k (nil : (Domain f s), tail)
+      | _ => k_fail f fds tail fs kind s k
       end.
 
 Ltac createLastInclusionTerm_dep dom f fds tail fs kind s k k_fail :=
   let is_equality := eval compute in (string_dec kind "InclusionIndex") in
       match is_equality with
-        | left _ =>
-          (findMatchingTerm
-             fds kind s
-             ltac:(fun X => k (fun x : dom => {| IndexSearchTerm := X x;
-                                                 ItemSearchTerm := tail x |}))
-                    || k (fun x : dom => {| IndexSearchTerm := nil;
-                                            ItemSearchTerm := tail x |}))
-        | _ => k_fail dom f fds tail fs kind s k
+      | left _ =>
+        (findMatchingTerm
+           fds kind s
+           ltac:(fun X => k (fun x : dom => (X x : (Domain f s), tail x )))
+                  || k (fun x : dom => (nil : (Domain f s), tail x)))
+      | _ => k_fail dom f fds tail fs kind s k
       end.
 
 Ltac createEarlyInclusionTerm f fds tail fs kind EarlyIndex LastIndex rest s k k_fail :=
   let is_equality := eval compute in (string_dec kind "InclusionIndex") in
       match is_equality with
-        | left _ =>
-          (findMatchingTerm
-             fds kind s
-             ltac:(fun X => k (X, rest)))
-            || k (@nil string, rest)
-        | _ => k_fail f fds tail fs kind EarlyIndex LastIndex rest s k
+      | left _ =>
+        (findMatchingTerm
+           fds kind s
+           ltac:(fun X => k (X, rest)))
+          || k (nil : (Domain f s), rest)
+      | _ => k_fail f fds tail fs kind EarlyIndex LastIndex rest s k
       end.
 
 Ltac createEarlyInclusionTerm_dep dom f fds tail fs kind EarlyIndex LastIndex rest s k k_fail :=
   let is_equality := eval compute in (string_dec kind "InclusionIndex") in
       match is_equality with
-        | left _ =>
-          (findMatchingTerm
-             fds kind s
-             ltac:(fun X => k (fun x : dom => (X x, rest x))))
-            || k (fun x : dom => (@nil string, rest x))
-        | _ => k_fail dom f fds tail fs kind EarlyIndex LastIndex rest s k
+      | left _ =>
+        (findMatchingTerm
+           fds kind s
+           ltac:(fun X => k (fun x : dom => (X x, rest x))))
+          || k (fun x : dom => (nil : (Domain f s), rest x))
+      | _ => k_fail dom f fds tail fs kind EarlyIndex LastIndex rest s k
       end.
 
 Ltac InclusionIndexTactics f :=
@@ -129,3 +113,46 @@ Ltac InclusionIndexTactics f :=
     matchInclusionIndex
     InclusionIndexUse createEarlyInclusionTerm createLastInclusionTerm
     InclusionIndexUse_dep createEarlyInclusionTerm_dep createLastInclusionTerm_dep f.
+
+Require Import
+        Coq.FSets.FMapInterface
+        Coq.FSets.FMapFacts
+        Coq.FSets.FMapAVL
+        Coq.Structures.OrderedTypeEx
+        Fiat.Common.String_as_OT
+        Fiat.QueryStructure.Implementation.DataStructures.Bags.InvertedIndexBags.
+
+Module StringInvertedIndexBag := InvertedIndexBag StringIndexedMap NatIndexedMap.
+Module NatInvertedIndexBag := InvertedIndexBag NatIndexedMap NatIndexedMap.
+Module NInvertedIndexBag := InvertedIndexBag NIndexedMap NatIndexedMap.
+Module ZInvertedIndexBag := InvertedIndexBag ZIndexedMap NatIndexedMap.
+
+    Ltac BuildLastInclusionIndexBag heading AttrList AttrKind AttrIndex k k_fail :=
+      let is_equality := eval compute in (string_dec AttrKind InclusionIndex) in
+          match is_equality with
+          | left _ =>
+            let AttrType := eval compute in (Domain heading AttrIndex) in
+                match AttrType with
+                | list string =>
+                  k (@StringInvertedIndexBag.InvertedIndexAsCorrectBag _ _                                                       (fun x => GetAttributeRaw (heading := heading) x AttrIndex)
+                                                                       (IndexedTreebupdate_transform heading)
+                    )
+
+                | list nat =>
+                  k (@NatInvertedIndexBag.InvertedIndexAsCorrectBag _ _                                                       (fun x => GetAttributeRaw (heading := heading) x AttrIndex)
+                                                                       (IndexedTreebupdate_transform heading)
+                    )
+
+                | list N =>
+                  k (@NInvertedIndexBag.InvertedIndexAsCorrectBag _ _                                                       (fun x => GetAttributeRaw (heading := heading) x AttrIndex)
+                                                                       (IndexedTreebupdate_transform heading)
+                    )
+
+                | list Z =>
+                  k (@ZInvertedIndexBag.InvertedIndexAsCorrectBag _ _                                                       (fun x => GetAttributeRaw (heading := heading) x AttrIndex)
+                                                                       (IndexedTreebupdate_transform heading)
+                    )
+
+                end
+          | right _ => k_fail heading AttrList AttrKind AttrIndex k
+          end.
